src/Ex/Mesi/MesiInvInv2.v
@@ -1,0 +1,988 @@
+Require Import Bool List String Peano_dec Lia.
+Require Import Common FMap IndexSupport HVector Syntax Topology Semantics SemFacts StepM.
+Require Import Invariant TrsInv Simulation Serial SerialFacts.
+Require Import RqRsLang RqRsInvMsg RqRsCorrect.
+
+Require Import Ex.Spec Ex.SpecInds Ex.Template.
+Require Import Ex.Mesi Ex.Mesi.Mesi Ex.Mesi.MesiTopo.
+
+Require Import Ex.Mesi.MesiInv Ex.Mesi.MesiInvInv0 Ex.Mesi.MesiInvInv1.
+
+Set Implicit Arguments.
+
+Import PropMonadNotations.
+Import CaseNotations.
+
+Local Open Scope list.
+Local Open Scope hvec.
+Local Open Scope fmap.
+
+Existing Instance Mesi.ImplOStateIfc.
+
+Definition ObjInvNotOwned (oidx: IdxT) (ost: OState) (msgs: MessagePool Msg) :=
+  ObjInvRq oidx msgs -> ost#[owned] = false.
+
+Definition InvNotOwned (st: MState): Prop :=
+  forall oidx,
+    ost <+- (bst_oss st)@[oidx]; ObjInvNotOwned oidx ost (bst_msgs st).
+
+Definition CohRsE (oidx: IdxT) (msgs: MessagePool Msg) (cv: nat) :=
+  MsgsP [((downTo oidx, (MRs, mesiRsE)),
+          (fun idm => (valOf idm).(msg_value) = cv))] msgs.
+
+Definition ObjCohDirE (ost: OState) :=
+  ost#[owned] = false /\
+  (mesiS <= ost#[status] \/ ost#[dir].(dir_st) = mesiE).
+
+Definition InvDirE (topo: DTree) (st: MState): Prop :=
+  forall oidx pidx,
+    parentIdxOf topo oidx = Some pidx ->
+    ost <+- (bst_oss st)@[oidx];
+      orq <+- (bst_orqs st)@[oidx];
+      post <+- (bst_oss st)@[pidx];
+      porq <+- (bst_orqs st)@[pidx];
+      (ObjDirE porq post oidx ->
+       (CohRsE oidx (bst_msgs st) post#[val] /\
+        (NoRsME oidx (bst_msgs st) ->
+         ObjCohDirE ost ->
+         post#[val] = ost#[val]))).
+
+Section InvDirE.
+  Variable (tr: tree).
+  Hypothesis (Htr: tr <> Node nil).
+
+  Let topo: DTree := fst (tree2Topo tr 0).
+  Let cifc: CIfc := snd (tree2Topo tr 0).
+  Let impl: System := impl Htr.
+
+  Lemma mesi_InvDirE_init:
+    Invariant.InvInit impl (InvDirE topo).
+  Proof.
+    do 2 (red; simpl); intros.
+    destruct (implOStatesInit tr)@[oidx] as [ost|] eqn:Host; simpl; auto.
+    destruct (implORqsInit tr)@[oidx] as [orq|] eqn:Horq; simpl; auto.
+    destruct (implOStatesInit tr)@[pidx] as [post|] eqn:Hpost; simpl; auto.
+    destruct (implORqsInit tr)@[pidx] as [porq|] eqn:Hporq; simpl; auto.
+    intros; exfalso.
+    red in H0; dest.
+    destruct (in_dec idx_dec pidx (c_li_indices cifc ++ c_l1_indices cifc)).
+    - subst cifc; rewrite c_li_indices_head_rootOf in i by assumption.
+      inv i.
+      + rewrite implOStatesInit_value_root in Hpost by assumption.
+        inv Hpost.
+        simpl in *; solve_mesi.
+      + rewrite implOStatesInit_value_non_root in Hpost by assumption.
+        inv Hpost.
+        simpl in *; solve_mesi.
+    - rewrite implOStatesInit_None in Hpost by assumption.
+      discriminate.
+  Qed.
+
+  Lemma mesi_InvDirE_ext_in:
+    forall oss orqs msgs,
+      InvDirE topo {| bst_oss := oss; bst_orqs := orqs; bst_msgs := msgs |} ->
+      InObjInds tr 0 {| bst_oss := oss; bst_orqs := orqs; bst_msgs := msgs |} ->
+      forall eins,
+        ValidMsgsExtIn impl eins ->
+        InvDirE topo {| bst_oss := oss;
+                        bst_orqs := orqs;
+                        bst_msgs := enqMsgs eins msgs |}.
+  Proof.
+    red; simpl; intros.
+    specialize (H _ _ H2); simpl in H.
+    destruct (oss@[oidx]) as [ost|] eqn:Host; simpl in *; auto.
+    destruct (orqs@[oidx]) as [orq|] eqn:Horq; simpl in *; auto.
+    destruct (oss@[pidx]) as [post|] eqn:Hpost; simpl in *; auto.
+    destruct (orqs@[pidx]) as [porq|] eqn:Hporq; simpl in *; auto.
+    intros; specialize (H H3); dest.
+    split.
+    - apply MsgsP_other_midx_enqMsgs; [assumption|].
+      destruct H1; simpl.
+      eapply DisjList_SubList; [eassumption|].
+      eapply DisjList_comm, DisjList_SubList.
+      + eapply SubList_trans;
+          [|eapply tree2Topo_obj_chns_minds_SubList with (oidx:= oidx)].
+        * solve_SubList.
+        * specialize (H0 oidx); simpl in H0.
+          rewrite Host in H0; simpl in H0.
+          eassumption.
+      + apply tree2Topo_minds_merqs_disj.
+    - intros; apply MsgsP_enqMsgs_inv in H5; auto.
+  Qed.
+
+  Lemma mesi_InvDirE_ext_out:
+    forall oss orqs msgs,
+      InvDirE topo {| bst_oss := oss; bst_orqs := orqs; bst_msgs := msgs |} ->
+      InObjInds tr 0 {| bst_oss := oss; bst_orqs := orqs; bst_msgs := msgs |} ->
+      forall (eouts: list (Id Msg)),
+        ValidMsgsExtOut impl eouts ->
+        InvDirE topo {| bst_oss := oss;
+                         bst_orqs := orqs;
+                         bst_msgs := deqMsgs (idsOf eouts) msgs |}.
+  Proof.
+    red; simpl; intros.
+    specialize (H _ _ H2); simpl in H.
+    destruct (oss@[oidx]) as [ost|] eqn:Host; simpl in *; auto.
+    destruct (orqs@[oidx]) as [orq|] eqn:Horq; simpl in *; auto.
+    destruct (oss@[pidx]) as [post|] eqn:Hpost; simpl in *; auto.
+    destruct (orqs@[pidx]) as [porq|] eqn:Hporq; simpl in *; auto.
+    intros; specialize (H H3); dest.
+    split.
+    - apply MsgsP_deqMsgs; assumption.
+    - intros; apply MsgsP_other_midx_deqMsgs_inv in H5; [auto|].
+      destruct H1.
+      simpl; eapply DisjList_SubList; [eassumption|].
+      eapply DisjList_comm, DisjList_SubList.
+      + eapply SubList_trans;
+          [|eapply tree2Topo_obj_chns_minds_SubList with (oidx:= oidx)].
+        * solve_SubList.
+        * specialize (H0 oidx); simpl in H0.
+          rewrite Host in H0; simpl in H0.
+          eassumption.
+      + apply tree2Topo_minds_merss_disj.
+  Qed.
+
+  Lemma InvDirE_enqMP:
+    forall oss orqs msgs,
+      InvDirE topo {| bst_oss:= oss; bst_orqs:= orqs; bst_msgs:= msgs |} ->
+      forall midx msg,
+        msg.(msg_id) <> mesiRsE ->
+        InvDirE topo {| bst_oss:= oss; bst_orqs:= orqs;
+                        bst_msgs:= enqMP midx msg msgs |}.
+  Proof.
+    red; simpl; intros.
+    specialize (H _ _ H1); simpl in H.
+    destruct (oss@[oidx]) as [ost|] eqn:Host; simpl in *; auto.
+    destruct (orqs@[oidx]) as [orq|] eqn:Horq; simpl in *; auto.
+    destruct (oss@[pidx]) as [post|] eqn:Hpost; simpl in *; auto.
+    destruct (orqs@[pidx]) as [porq|] eqn:Hporq; simpl in *; auto.
+    intros; specialize (H H2); dest.
+    split.
+    - apply MsgsP_other_msg_id_enqMP; [assumption|].
+      simpl; intro Hx; destruct Hx; auto.
+    - intros; apply MsgsP_enqMP_inv in H4; auto.
+  Qed.
+  
+  Lemma InvDirE_enqMsgs:
+    forall oss orqs msgs,
+      InvDirE topo {| bst_oss:= oss; bst_orqs:= orqs; bst_msgs:= msgs |} ->
+      forall nmsgs,
+        Forall (fun idm => (valOf idm).(msg_id) <> mesiRsE) nmsgs ->
+        InvDirE topo {| bst_oss:= oss; bst_orqs:= orqs;
+                        bst_msgs:= enqMsgs nmsgs msgs |}.
+  Proof.
+    intros.
+    generalize dependent msgs.
+    induction nmsgs as [|[nmidx nmsg] nmsgs]; simpl; intros; auto.
+    inv H0.
+    apply IHnmsgs; auto.
+    apply InvDirE_enqMP; assumption.
+  Qed.
+
+  Lemma InvDirE_deqMP:
+    forall oss orqs msgs,
+      InvDirE topo {| bst_oss:= oss; bst_orqs:= orqs; bst_msgs:= msgs |} ->
+      forall midx msg,
+        FirstMP msgs midx msg ->
+        msg.(msg_id) <> mesiRsM ->
+        msg.(msg_id) <> mesiRsE ->
+        InvDirE topo {| bst_oss:= oss; bst_orqs:= orqs;
+                        bst_msgs:= deqMP midx msgs |}.
+  Proof.
+    unfold InvDirE; simpl; intros.
+    specialize (H _ _ H3).
+    destruct (oss@[oidx]) as [ost|] eqn:Host; simpl in *; auto.
+    destruct (orqs@[oidx]) as [orq|] eqn:Horq; simpl in *; auto.
+    destruct (oss@[pidx]) as [post|] eqn:Hpost; simpl in *; auto.
+    destruct (orqs@[pidx]) as [porq|] eqn:Hporq; simpl in *; auto.
+    intros; specialize (H H4); dest.
+    split.
+    - apply MsgsP_deqMP; assumption.
+    - intros; eapply MsgsP_other_msg_id_deqMP_inv in H6;
+        [|eassumption|simpl; intro; intuition].
+      auto.
+  Qed.
+
+  Lemma InvDirE_deqMsgs:
+    forall oss orqs msgs,
+      InvDirE topo {| bst_oss:= oss; bst_orqs:= orqs; bst_msgs:= msgs |} ->
+      forall rmsgs,
+        Forall (FirstMPI msgs) rmsgs ->
+        NoDup (idsOf rmsgs) ->
+        Forall (fun idm => (valOf idm).(msg_id) <> mesiRsM /\
+                           (valOf idm).(msg_id) <> mesiRsE) rmsgs ->
+        InvDirE topo {| bst_oss:= oss; bst_orqs:= orqs;
+                        bst_msgs:= deqMsgs (idsOf rmsgs) msgs |}.
+  Proof.
+    unfold InvDirE; simpl; intros.
+    specialize (H _ _ H3).
+    destruct (oss@[oidx]) as [ost|] eqn:Host; simpl in *; auto.
+    destruct (orqs@[oidx]) as [orq|] eqn:Horq; simpl in *; auto.
+    destruct (oss@[pidx]) as [post|] eqn:Hpost; simpl in *; auto.
+    destruct (orqs@[pidx]) as [porq|] eqn:Hporq; simpl in *; auto.
+    intros; specialize (H H4); dest.
+    split.
+    - apply MsgsP_deqMsgs; assumption.
+    - intros; eapply MsgsP_other_msg_id_deqMsgs_inv in H6; try eassumption.
+      + specialize (H5 H6 H7); dest; auto.
+      + simpl.
+        apply (DisjList_spec_1 idx_dec); intros.
+        apply in_map_iff in H8; destruct H8 as [idm [? ?]].
+        rewrite Forall_forall in H2; specialize (H2 _ H9); dest; subst.
+        intro; dest_in; auto.
+  Qed.
+
+  Ltac solve_msg :=
+    simpl;
+    try match goal with
+        | [H: msg_id ?rmsg = _ |- msg_id ?rmsg <> _] => rewrite H
+        end;
+    discriminate.
+
+  Ltac solve_enqMsgs :=
+    let idm := fresh "idm" in
+    let Hin := fresh "H" in
+    apply Forall_forall; intros idm Hin;
+    apply in_map_iff in Hin; dest; subst;
+    solve_msg.
+
+  Ltac solve_deqMsgs_NoDup :=
+    match goal with
+    | [H: ValidMsgsIn _ ?msgs |- NoDup (idsOf ?msgs)] => apply H
+    end.
+
+  Ltac solve_deqMsgs_msg_id :=
+    match goal with
+    | [H: Forall (fun _ => msg_id _ = _) ?msgs |- Forall _ ?msgs] =>
+      eapply Forall_impl; [|eapply H];
+      simpl; intros; split; solve_msg
+    end.
+
+  Ltac simpl_InvDirE_msgs :=
+    repeat
+      (first [apply InvDirE_enqMP; [|solve_msg..]
+             |apply InvDirE_enqMsgs; [|solve_enqMsgs]
+             |eapply InvDirE_deqMP; [|eassumption|solve_msg..]
+             |apply InvDirE_deqMsgs; [|eassumption
+                                      |solve_deqMsgs_NoDup
+                                      |solve_deqMsgs_msg_id]
+             |assumption]).
+
+  Ltac disc_bind_true :=
+    repeat
+      match goal with
+      | |- _ <+- ?ov; _ =>
+        first [match goal with
+               | [H: ov = _ |- _] => rewrite H in *; simpl in *
+               end
+              |let Hov := fresh "H" in
+               let v := fresh "v" in
+               destruct ov as [v|] eqn:Hov; simpl in *; [|auto]]
+      end.
+
+  Ltac disc_ObjDirE :=
+    match goal with
+    | [H: ObjDirE _ _ _ |- _] =>
+      red in H; simpl in H; dest; subst
+    end.
+
+  Ltac disc_NoRsME :=
+    repeat
+      match goal with
+      | [H: ValidMsgsIn _ _ |- _] => destruct H
+      | [H: ValidMsgsOut _ _ |- _] => destruct H
+      end;
+    repeat
+      match goal with
+      | [H: NoRsME _ _ |- _] => disc_MsgsP H
+      | [Hi: NoRsME _ ?msgs -> _ /\ _,  Hm: MsgsP _ ?msgs |- _] =>
+        specialize (Hi Hm); dest
+      end.
+
+  Ltac disc :=
+    repeat
+      match goal with
+      | [Hi: InvDirE _ _ |- InvDirE _ _] =>
+        let Hp := fresh "H" in
+        red; simpl; intros ? ? Hp;
+        specialize (Hi _ _ Hp); simpl in Hi;
+        mred; simpl;
+        try (exfalso; eapply parentIdxOf_not_eq; subst topo; eauto; fail)
+      | |- _ <+- _; _ => disc_bind_true
+      | |- _ -> _ => intros
+      | [Hi: ObjDirE _ _ _ -> _, Ho: ObjDirE _ _ _ |- _] =>
+        specialize (Hi Ho); dest
+      | [Hi: NoRsME _ _ -> _, Hm: NoRsME _ _ |- _] =>
+        specialize (Hi Hm)
+      | [Hi: ObjCohDirE ?ost -> _, Hm: ObjCohDirE ?ost |- _] =>
+        specialize (Hi Hm)
+      | [H: ?t = ?t -> _ |- _] => specialize (H eq_refl); dest
+      end.
+
+  Ltac solve_by_diff_dir :=
+    intros;
+    match goal with
+    | [Hn: ObjDirE _ _ _ |- _] =>
+      red in Hn; dest; simpl in *; solve_mesi
+    end.
+
+  Ltac solve_by_idx_false :=
+    intros; subst topo; congruence.
+
+  Ltac solve_by_NoRsME_false :=
+    exfalso;
+    match goal with
+    | [Hn: NoRsME _ (enqMP ?midx ?msg ?msgs) |- _] =>
+      specialize (Hn (midx, msg)
+                     (InMP_or_enqMP
+                        msgs (or_introl (conj eq_refl eq_refl))));
+      red in Hn; unfold map in Hn;
+      disc_caseDec Hn; auto
+    end.
+
+  Ltac solve_ObjCohDirE :=
+    try assumption;
+    match goal with
+    | [H: ObjCohDirE _ |- _] =>
+      red in H; dest; red; simpl in *
+    end; intuition solve_mesi.
+
+  Ltac solve_coh :=
+    intros;
+    match goal with
+    | [H: _ -> _ -> fst ?lv = fst ?rv |- fst ?lv = fst ?rv] =>
+      apply H; [disc_NoRsME; assumption|solve_ObjCohDirE]
+    end.
+
+  Ltac solve_by_ObjCohDirE_false :=
+    intros;
+    match goal with
+    | [H: ObjCohDirE _ |- _] =>
+      red in H; simpl in *; dest; solve [discriminate|solve_mesi]
+    end.
+
+  Ltac solve_valid :=
+    split; [solve_MsgsP|solve_coh].
+
+  Lemma mesi_InvDirE_step:
+    Invariant.InvStep impl step_m (InvDirE topo).
+  Proof. (* SKIP_PROOF_OFF *)
+    red; intros.
+    pose proof (footprints_ok
+                  (mesi_GoodORqsInit Htr)
+                  (mesi_GoodRqRsSys Htr) H) as Hftinv.
+    pose proof (mesi_InObjInds H) as Hioi.
+    pose proof (mesi_MsgConflictsInv
+                  (@mesi_RootChnInv_ok _ Htr) H) as Hpmcf.
+    pose proof (mesi_InvWBDir_ok H) as Hwd.
+    pose proof (MesiDownLockInv_ok H) as Hmdl.
+    pose proof (mesi_InvL1DirI_ok H) as Hl1d.
+    pose proof (mesi_InvDirME_ok H) as Hdme.
+    inv H1; [assumption
+            |apply mesi_InvDirE_ext_in; auto
+            |apply mesi_InvDirE_ext_out; auto
+            |].
+
+    simpl in H2; destruct H2; [subst|apply in_app_or in H1; destruct H1].
+    
+    - (*! Cases for the main memory *)
+
+      (** Abstract the root. *)
+      assert (In (rootOf (fst (tree2Topo tr 0)))
+                 (c_li_indices (snd (tree2Topo tr 0)))) as Hin.
+      { rewrite c_li_indices_head_rootOf by assumption.
+        left; reflexivity.
+      }
+
+      remember (rootOf (fst (tree2Topo tr 0))) as oidx; clear Heqoidx.
+
+      (** Do case analysis per a rule. *)
+      apply in_app_or in H3; destruct H3.
+
+      1: { (** Rules per a child *)
+        apply concat_In in H1; destruct H1 as [crls [? ?]].
+        apply in_map_iff in H1; destruct H1 as [cidx [? ?]]; subst.
+
+        (** Derive that the child has the parent. *)
+        assert (parentIdxOf (fst (tree2Topo tr 0)) cidx = Some oidx)
+          by (apply subtreeChildrenIndsOf_parentIdxOf; auto).
+
+        dest_in.
+
+        { (* [liGetSImmS] *)
+          disc_rule_conds_ex; disc.
+          { solve_valid. }
+          { solve_by_diff_dir. }
+          { destruct (idx_dec cidx oidx0); subst.
+            { solve_by_idx_false. }
+            { solve_valid. }
+          }
+        }
+        
+        { (* [liGetSImmME] *)
+          disc_rule_conds_ex; disc.
+          { solve_valid. }
+          { disc_ObjDirE.
+            split; intros.
+            { apply MsgsP_enqMP.
+              { admit. (** TODO: since [RsE] is already there .. *) }
+              { red; unfold map.
+                rewrite caseDec_head_eq by reflexivity.
+                reflexivity.
+              }
+            }
+            { solve_by_NoRsME_false. }
+          }
+          { destruct (idx_dec cidx oidx0); subst.
+            { solve_by_idx_false. }
+            { solve_valid. }
+          }
+        }
+
+        { (* [liGetSRqUpDownME] *)
+          disc_rule_conds_ex; simpl_InvDirE_msgs; disc.
+          disc_ObjDirE; mred.
+        }
+
+        { (* [liGetMImm] *)
+          disc_rule_conds_ex; disc.
+          { solve_valid. }
+          { solve_by_diff_dir. }
+          { destruct (idx_dec cidx oidx0); subst.
+            { solve_by_idx_false. }
+            { solve_valid. }
+          }
+        }
+
+        { (* [liGetMRqUpDownME] *)
+          disc_rule_conds_ex; simpl_InvDirE_msgs; disc.
+          disc_ObjDirE; mred.
+        }
+        { (* [liGetMRqUpDownS] *)
+          disc_rule_conds_ex; simpl_InvDirE_msgs; disc.
+          disc_ObjDirE; mred.
+        }
+
+        { (* [liInvImmI] *)
+          disc_rule_conds_ex; simpl_InvDirE_msgs; disc.
+        }
+
+        { (* [liInvImmS0] *)
+          disc_rule_conds_ex; simpl_InvDirE_msgs; disc.
+          { solve_valid. }
+          { solve_by_diff_dir. }
+        }
+
+        { (* [liInvImmS1] *)
+          disc_rule_conds_ex; simpl_InvDirE_msgs; disc.
+          { solve_valid. }
+          { solve_by_diff_dir. }
+        }
+
+        { (* [liInvImmE] *)
+          disc_rule_conds_ex; simpl_InvDirE_msgs; disc.
+          { split; [solve_MsgsP|disc_getDir; solve_coh]. }
+          { solve_by_diff_dir. }
+        }
+
+        { (* [liInvImmWBI] *)
+          disc_rule_conds_ex; simpl_InvDirE_msgs; disc.
+        }
+
+        { (* [liInvImmWBS1] *)
+          disc_rule_conds_ex; simpl_InvDirE_msgs; disc.
+          { solve_valid. }
+          { solve_by_diff_dir. }
+        }
+
+        { (* [liInvImmWBME] *)
+          disc_rule_conds_ex; simpl_InvDirE_msgs; disc.
+          { split; [solve_MsgsP|solve_by_ObjCohDirE_false]. }
+          { solve_by_diff_dir. }
+        }
+
+      }
+
+      dest_in.
+
+      { (* [liDownSRsUpDownME] *)
+        disc_rule_conds_ex.
+        disc_MesiDownLockInv oidx Hmdl.
+        simpl_InvDirE_msgs; disc.
+        { split; [solve_MsgsP|solve_by_ObjCohDirE_false]. }
+        { solve_by_diff_dir. }
+      }
+
+      { (* [liDownIRsUpDown] *)
+        disc_rule_conds_ex.
+        disc_MesiDownLockInv oidx Hmdl.
+        simpl_InvDirE_msgs; disc.
+        { solve_valid. }
+        { solve_by_diff_dir. }
+      }        
+
+    - (*! Cases for Li caches *)
+
+      (** Derive some necessary information: each Li has a parent. *)
+      apply in_map_iff in H1; destruct H1 as [oidx [? ?]]; subst; simpl in *.
+
+      pose proof (tree2Topo_TreeTopoNode tr 0) as Htn.
+      pose proof (c_li_indices_tail_has_parent Htr _ _ H2).
+      destruct H1 as [pidx [? ?]].
+      pose proof (Htn _ _ H4); dest.
+
+      (** Do case analysis per a rule. *)
+      apply in_app_or in H3; destruct H3.
+
+      1: { (** Rules per a child *)
+        apply concat_In in H3; destruct H3 as [crls [? ?]].
+        apply in_map_iff in H3; destruct H3 as [cidx [? ?]]; subst.
+
+        (** Derive that the child has the parent. *)
+        assert (parentIdxOf (fst (tree2Topo tr 0)) cidx = Some oidx)
+          by (apply subtreeChildrenIndsOf_parentIdxOf; auto).
+
+        dest_in.
+
+        { (* [liGetSImmS] *)
+          disc_rule_conds_ex; disc.
+          { solve_valid. }
+          { solve_by_diff_dir. }
+          { destruct (idx_dec cidx oidx0); subst.
+            { solve_by_idx_false. }
+            { solve_valid. }
+          }
+        }
+
+        { (* [liGetSImmME] *)
+          disc_rule_conds_ex; disc.
+          { solve_valid. }
+          { disc_ObjDirE.
+            split; intros.
+            { apply MsgsP_enqMP.
+              { admit. (** TODO: since [RsE] is already there .. *) }
+              { red; unfold map.
+                rewrite caseDec_head_eq by reflexivity.
+                reflexivity.
+              }
+            }
+            { solve_by_NoRsME_false. }
+          }
+          { destruct (idx_dec cidx oidx0); subst.
+            { solve_by_idx_false. }
+            { solve_valid. }
+          }
+        }
+
+        { (* [liGetSRqUpUp] *)
+          disc_rule_conds_ex; simpl_InvDirE_msgs.
+          disc; red in H18; mred.
+          specialize (H0 H18); dest.
+          solve_valid.
+        }
+
+        { (* [liGetSRqUpDownME] *)
+          disc_rule_conds_ex; simpl_InvDirE_msgs; disc.
+          disc_ObjDirE; mred.
+        }
+
+        { (* [liGetMImm] *)
+          disc_rule_conds_ex; disc.
+          { solve_valid. }
+          { solve_by_diff_dir. }
+          { destruct (idx_dec cidx oidx0); subst.
+            { solve_by_idx_false. }
+            { solve_valid. }
+          }
+        }
+
+        { (* [liGetMRqUpUp] *)
+          disc_rule_conds_ex; simpl_InvDirE_msgs.
+          disc; red in H18; mred.
+          specialize (H0 H18); dest.
+          solve_valid.
+        }
+
+        { (* [liGetMRqUpDownME] *)
+          disc_rule_conds_ex; simpl_InvDirE_msgs; disc.
+          disc_ObjDirE; mred.
+        }
+        { (* [liGetMRqUpDownS] *)
+          disc_rule_conds_ex; simpl_InvDirE_msgs; disc.
+          disc_ObjDirE; mred.
+        }
+
+        { (* [liInvImmI] *)
+          disc_rule_conds_ex; simpl_InvDirE_msgs; disc.
+        }
+
+        { (* [liInvImmS0] *)
+          disc_rule_conds_ex; simpl_InvDirE_msgs; disc.
+          { solve_valid. }
+          { solve_by_diff_dir. }
+        }
+
+        { (* [liInvImmS1] *)
+          disc_rule_conds_ex; simpl_InvDirE_msgs; disc.
+          { solve_valid. }
+          { solve_by_diff_dir. }
+        }
+
+        { (* [liInvImmE] *)
+          disc_rule_conds_ex; simpl_InvDirE_msgs; disc.
+          { split; [solve_MsgsP|disc_getDir; solve_coh]. }
+          { solve_by_diff_dir. }
+        }
+
+        { (* [liInvImmWBI] *)
+          disc_rule_conds_ex; simpl_InvDirE_msgs; disc.
+        }
+
+        { (* [liInvImmWBS1] *)
+          disc_rule_conds_ex; simpl_InvDirE_msgs; disc.
+          { solve_valid. }
+          { solve_by_diff_dir. }
+        }
+
+        { (* [liInvImmWBME] *)
+          disc_rule_conds_ex; simpl_InvDirE_msgs; disc.
+          { split; [solve_MsgsP|solve_by_ObjCohDirE_false]. }
+          { solve_by_diff_dir. }
+        }
+
+      }
+
+      dest_in.
+
+      { (* [liGetSRsDownDownS] *)
+        disc_rule_conds_ex.
+        derive_footprint_info_basis oidx.
+        derive_child_chns cidx.
+        disc_rule_conds_ex.
+        disc.
+        { (** TODO: need to have [InvDirME]? *)
+          admit.
+        }
+        { solve_by_diff_dir. }
+        { destruct (idx_dec cidx oidx0); subst.
+          { solve_by_idx_false. }
+          { solve_valid. }
+        }
+      }
+
+      { (* [liGetSRsDownDownE] *)
+        disc_rule_conds_ex.
+        derive_footprint_info_basis oidx.
+        derive_child_chns cidx.
+        disc_rule_conds_ex.
+        disc.
+        { split; [solve_MsgsP|].
+          (* pulling a coherence value from the [mesiRsE] message. *)
+          intros.
+          move H0 at bottom.
+          specialize (H0 _ (FirstMP_InMP H21)).
+          red in H0.
+          unfold map in H0.
+          rewrite caseDec_head_eq in H0 by (unfold sigOf; simpl; congruence).
+          auto.
+        }
+        { disc_ObjDirE.
+          split; intros.
+          { apply MsgsP_enqMP.
+            { admit. (** TODO: since [RsE] is already there .. *) }
+            { red; unfold map.
+              rewrite caseDec_head_eq by reflexivity.
+              reflexivity.
+            }
+          }
+          { solve_by_NoRsME_false. }
+        }
+        { destruct (idx_dec cidx oidx0); subst.
+          { solve_by_idx_false. }
+          { solve_valid. }
+        }
+      }
+
+      { (* [liDownSRsUpDownME] *)
+        disc_rule_conds_ex; simpl_InvDirE_msgs; disc.
+        { split; [solve_MsgsP|solve_by_ObjCohDirE_false]. }
+        { solve_by_diff_dir. }
+      }
+
+      { (* [liDownSImm] *)
+        disc_rule_conds_ex; simpl_InvDirE_msgs; disc.
+        exfalso.
+        subst topo; disc_rule_conds_ex.
+        disc_ObjDirE.
+        remember (dir_excl _) as oidx; clear Heqoidx.
+        derive_parent_downlock_by_RqDown oidx.
+        auto.
+      }
+
+      { (* [liDownSRqDownDownME] *)
+        disc_rule_conds_ex; simpl_InvDirE_msgs; disc.
+        disc_ObjDirE; mred.
+      }
+
+      { (* [liDownSRsUpUp] *)
+        disc_rule_conds_ex.
+        disc_MesiDownLockInv oidx Hmdl.
+        simpl_InvDirE_msgs; disc.
+        { disc_ObjDirE.
+          remember (dir_excl _) as oidx; clear Heqoidx.
+          disc_MsgConflictsInv oidx.
+
+          Ltac solve_by_child_downlock_to_parent oidx :=
+            exfalso;
+            disc_MsgConflictsInv oidx;
+            match goal with
+            | [Hp: ParentLockFreeConflicts oidx ?porq ?orq,
+                   Ho: ?orq@[downRq] = None,
+                       Hpo: ?porq@[downRq] = Some _ |- _] =>
+              specialize (Hp Ho); rewrite Hpo in Hp;
+              simpl in Hp; auto
+            end.
+
+          solve_by_child_downlock_to_parent oidx.
+        }
+        { solve_by_diff_dir. }
+      }
+
+      { (* [liGetMRsDownDownDirI] *)
+        disc_rule_conds_ex.
+        derive_footprint_info_basis oidx.
+        derive_child_chns cidx.
+        disc_rule_conds_ex.
+        disc.
+        { split; [solve_MsgsP|solve_by_ObjCohDirE_false]. }
+        { solve_by_diff_dir. }
+        { destruct (idx_dec cidx oidx0); subst.
+          { solve_by_idx_false. }
+          { solve_valid. }
+        }
+      }
+
+      { (* [liGetMRsDownRqDownDirS] *)
+        disc_rule_conds_ex.
+        derive_footprint_info_basis oidx.
+        simpl_InvDirE_msgs; disc.
+        { split; [solve_MsgsP|solve_by_ObjCohDirE_false]. }
+        { solve_by_diff_dir. }
+        { solve_valid. }
+      }
+      
+      { (* [liDownIRsUpDown] *)
+        disc_rule_conds_ex.
+        disc_MesiDownLockInv oidx Hmdl.
+        simpl_InvDirE_msgs; disc.
+        { solve_valid. }
+        { solve_by_diff_dir. }
+      }
+
+      { (* [liDownIImm] *)
+        disc_rule_conds_ex; simpl_InvDirE_msgs; disc.
+        exfalso.
+        subst topo; disc_rule_conds_ex.
+        disc_ObjDirE.
+        remember (dir_excl _) as oidx; clear Heqoidx.
+        derive_parent_downlock_by_RqDown oidx.
+        auto.
+      }
+
+      { (* [liDownIRqDownDownDirS] *)
+        disc_rule_conds_ex; simpl_InvDirE_msgs; disc.
+        disc_ObjDirE; mred.
+      }
+      { (* [liDownIRqDownDownDirME] *)
+        disc_rule_conds_ex; simpl_InvDirE_msgs; disc.
+        disc_ObjDirE; mred.
+      }
+
+      { (* [liDownIRsUpUp] *)
+        disc_rule_conds_ex.
+        disc_MesiDownLockInv oidx Hmdl.
+        simpl_InvDirE_msgs; disc.
+        { subst topo; disc_rule_conds_ex.
+          disc_ObjDirE.
+          remember (dir_excl _) as oidx; clear Heqoidx.
+          disc_MsgConflictsInv oidx.
+          solve_by_child_downlock_to_parent oidx.
+        }
+        { solve_by_diff_dir. }
+      }
+
+      { (* [liInvRqUpUp] *)
+        disc_rule_conds_ex; simpl_InvDirE_msgs; disc.
+        disc_ObjDirE; solve_mesi.
+      }
+
+      { (* [liInvRqUpUpWB] *)
+        disc_rule_conds_ex; simpl_InvDirE_msgs; disc.
+        disc_ObjDirE; solve_mesi.
+      }
+
+      { (* [liInvRsDownDown] *)
+        disc_rule_conds_ex.
+        derive_footprint_info_basis oidx.
+        derive_InvWBDir oidx.
+        assert (ObjInvRs oidx msgs) as Hirs.
+        { do 2 red.
+          eexists; split; [apply FirstMP_InMP; eassumption|].
+          unfold sigOf; simpl; congruence.
+        }
+        specialize (Hwd (or_intror (or_intror Hirs))); clear Hirs.
+
+        simpl_InvDirE_msgs; disc.
+        { split; [solve_MsgsP|solve_by_ObjCohDirE_false]. }
+        { disc_ObjDirE; solve_mesi. }
+      }
+
+      { (* [liPushImm] *)
+        disc_rule_conds_ex; disc; solve_valid.
+      }
+      
+    - (*! Cases for L1 caches *)
+
+      (** Derive some necessary information: each Li has a parent. *)
+      apply in_map_iff in H1; destruct H1 as [oidx [? ?]]; subst.
+
+      pose proof (tree2Topo_TreeTopoNode tr 0) as Htn.
+      pose proof (c_l1_indices_has_parent Htr _ _ H2).
+      destruct H1 as [pidx [? ?]].
+      pose proof (Htn _ _ H4); dest.
+
+      (** Discharge an invariant that holds only for L1 caches. *)
+      red in Hl1d; simpl in Hl1d.
+      rewrite Forall_forall in Hl1d; specialize (Hl1d _ H2).
+      simpl in H5; rewrite H5 in Hl1d; simpl in Hl1d.
+
+      (** Do case analysis per a rule. *)
+      dest_in.
+
+      { disc_rule_conds_ex; simpl_InvDirE_msgs; disc. }
+
+      { disc_rule_conds_ex; simpl_InvDirE_msgs; disc.
+        red in H16; mred; specialize (H0 H16); dest.
+        solve_valid.
+      }
+      
+      { disc_rule_conds_ex; simpl_InvDirE_msgs.
+        derive_footprint_info_basis oidx.
+        derive_child_chns cidx.
+        disc_rule_conds_ex.
+        disc.
+        { (** TODO: need to have [InvDirME]. *)
+          admit.
+        }
+        { solve_by_diff_dir. }
+      }
+
+      { disc_rule_conds_ex.
+        disc_rule_conds_ex.
+        derive_footprint_info_basis oidx.
+        derive_child_chns cidx.
+        disc_rule_conds_ex.
+        disc.
+        { split; [solve_MsgsP|].
+          (* pulling a coherence value from the [mesiRsE] message. *)
+          intros.
+          move H0 at bottom.
+          specialize (H0 _ (FirstMP_InMP H21)).
+          red in H0.
+          unfold map in H0.
+          rewrite caseDec_head_eq in H0 by (unfold sigOf; simpl; congruence).
+          auto.
+        }
+        { disc_ObjDirE; solve_mesi. }
+        { destruct (idx_dec (l1ExtOf oidx) oidx0); subst.
+          { exfalso.
+            subst topo.
+            rewrite tree2Topo_l1_ext_parent in H3 by assumption.
+            congruence.
+          }
+          { solve_valid. }
+        }
+      }
+
+      { disc_rule_conds_ex; simpl_InvDirE_msgs; disc.
+        exfalso.
+        subst topo; disc_rule_conds_ex.
+        disc_ObjDirE.
+        remember (dir_excl _) as oidx; clear Heqoidx.
+        derive_parent_downlock_by_RqDown oidx.
+        auto.
+      }
+
+      { disc_rule_conds_ex; simpl_InvDirE_msgs; disc.
+        { split; [solve_MsgsP|solve_by_ObjCohDirE_false]. }
+        { solve_by_diff_dir. }
+      }
+
+      { disc_rule_conds_ex; simpl_InvDirE_msgs; disc.
+        { split; [solve_MsgsP|].
+          admit. (** TODO: well we know [owned = T] here.. *)
+        }
+        { solve_by_diff_dir. }
+      }
+
+      { disc_rule_conds_ex; simpl_InvDirE_msgs.
+        disc; red in H16; mred.
+        specialize (H0 H16); dest.
+        solve_valid.
+      }
+
+      { disc_rule_conds_ex.
+        derive_footprint_info_basis oidx.
+        derive_child_chns cidx.
+        disc_rule_conds_ex.
+        disc.
+        { split; [solve_MsgsP|solve_by_ObjCohDirE_false]. }
+        { solve_by_diff_dir. }
+        { destruct (idx_dec (l1ExtOf oidx) oidx0); subst.
+          { exfalso.
+            subst topo.
+            rewrite tree2Topo_l1_ext_parent in H3 by assumption.
+            congruence.
+          }
+          { solve_valid. }
+        }
+      }
+
+      { disc_rule_conds_ex; simpl_InvDirE_msgs; disc.
+        exfalso.
+        subst topo; disc_rule_conds_ex.
+        disc_ObjDirE.
+        remember (dir_excl _) as oidx; clear Heqoidx.
+        derive_parent_downlock_by_RqDown oidx.
+        auto.
+      }
+
+      { disc_rule_conds_ex; simpl_InvDirE_msgs; disc.
+        disc_ObjDirE; solve_mesi.
+      }
+
+      { disc_rule_conds_ex; simpl_InvDirE_msgs; disc.
+        disc_ObjDirE; solve_mesi.
+      }
+
+      { (* [liInvRsDownDown] *)
+        disc_rule_conds_ex.
+        derive_footprint_info_basis oidx.
+        derive_InvWBDir oidx.
+        assert (ObjInvRs oidx msgs) as Hirs.
+        { do 2 red.
+          eexists; split; [apply FirstMP_InMP; eassumption|].
+          unfold sigOf; simpl; congruence.
+        }
+        specialize (Hwd (or_intror (or_intror Hirs))); clear Hirs.
+
+        simpl_InvDirE_msgs; disc.
+        { split; [solve_MsgsP|solve_by_ObjCohDirE_false]. }
+        { disc_ObjDirE; solve_mesi. }
+      }
+      
+      (* END_SKIP_PROOF_OFF *)
+  Qed.
+
+End InvDirE.
+  
